verification/tests/ShadowingFix.fst
@@ -1,8 +1,4 @@
-(** Shadowing Bug -- FIXED
-    
-    slot_of now scans right-to-left (returns LAST occurrence).
-    Expression: (let [x 1] (let [x 2] x)) -> should evaluate to 2.
-*)
+(** Shadowing Bug -- FIXED *)
 module ShadowingFix
 
 open Lisp.Types
@@ -11,51 +7,44 @@ open Lisp.Source
 open Lisp.Compiler
 open LispIR.Semantics
 
-val shadowing_expr : lisp_val
-let shadowing_expr = List [
-  Sym "let";
-  List [List [Sym "x"; Num 1]];
-  List [
-    Sym "let";
-    List [List [Sym "x"; Num 2]];
-    Sym "x"
-  ]
-]
-
 val slot_of_finds_correct : unit -> Lemma
-  (match slot_of "x" ["x"; "x"] with
-   | Some 1 -> true
-   | _ -> false)
+  (match slot_of "x" ["x"; "x"] with | Some 1 -> true | _ -> false)
 let slot_of_finds_correct () = ()
 
 val slot_of_non_shadowed : unit -> Lemma
-  (match slot_of "x" ["x"; "y"] with
-   | Some 0 -> true
-   | _ -> false)
+  (match slot_of "x" ["x"; "y"] with | Some 0 -> true | _ -> false)
 let slot_of_non_shadowed () = ()
 
 val slot_of_single : unit -> Lemma
-  (match slot_of "x" ["x"] with
-   | Some 0 -> true
-   | _ -> false)
+  (match slot_of "x" ["x"] with | Some 0 -> true | _ -> false)
 let slot_of_single () = ()
 
-val compiler_produces_fixed_code : unit -> Lemma (true)
-let compiler_produces_fixed_code () = admit ()
+val slot_of_triple : unit -> Lemma
+  (match slot_of "x" ["x"; "x"; "x"] with | Some 2 -> true | _ -> false)
+let slot_of_triple () = ()
 
 val vm_gives_correct_2 : unit -> Lemma
-  (let s = { stack = []; slots = []; pc = 0;
-             code = [PushI64 1; StoreSlot 0; PushI64 2; StoreSlot 1; LoadSlot 1; Return];
-             ok = true } in
-   match eval_steps 100 s with
-   | Ok s' -> (match s'.stack with
-     | Num 2 :: _ -> true
-     | _ -> false)
+  (match eval_steps 100 { stack = []; slots = []; pc = 0;
+    code = [PushI64 1; StoreSlot 0; PushI64 2; StoreSlot 1; LoadSlot 1; Return];
+    ok = true } with
+   | Ok s' -> (match s'.stack with Num 2 :: _ -> true | _ -> false)
    | _ -> false)
 let vm_gives_correct_2 () = ()
 
-val slot_of_triple : unit -> Lemma
-  (match slot_of "x" ["x"; "x"; "x"] with
-   | Some 2 -> true
-   | _ -> false)
-let slot_of_triple () = ()
+// Step 1: inner let (let [x 2] x) compiles with slot_map ["x"]
+val inner_let_spec : fuel:int -> Lemma
+  (fuel > 10 ==> (match compile_lambda fuel ["x"]
+    (List [Sym "let"; List [List [Sym "x"; Num 2]]; Sym "x"]) with
+   | Some [PushI64 2; StoreSlot 1; LoadSlot 1; Return] -> true
+   | _ -> false))
+let inner_let_spec fuel = ()
+
+// Step 2: outer let (let [x 1] INNER) compiles with slot_map []
+// This chains inner + outer -- the admit
+val compiler_produces_fixed_code : fuel:int -> Lemma
+  (fuel > 10 ==> (match compile_lambda fuel []
+    (List [Sym "let"; List [List [Sym "x"; Num 1]];
+      List [Sym "let"; List [List [Sym "x"; Num 2]]; Sym "x"]]) with
+   | Some [PushI64 1; StoreSlot 0; PushI64 2; StoreSlot 1; LoadSlot 1; Return] -> true
+   | _ -> false))
+let compiler_produces_fixed_code fuel = admit ()
